@base <http://apps4eu.eu/odapps#>.

@prefix org: <http://www.w3.org/ns/org#>.
@prefix rdfs: <http://www.w3.org/2000/01/rdf-schema#>.
@prefix rdf: <http://www.w3.org/1999/02/22-rdf-syntax-ns#>.
@prefix foaf: <http://xmlns.com/foaf/0.1/>.
@prefix odapps: <http://apps4europe.eu/vocab/odapps#>.
@prefix apps4eu: <http://apps4europe.eu/vocab/apps4X#>.
@prefix owl: <http://www.w3.org/2002/07/owl#>.
@prefix dvia: <http://data.eurecom.fr/ontology/dvia#>.
@prefix schema: <http://schema.org/> .
@prefix dcat: <http://www.w3.org/ns/dcat#> .
@prefix dct: <http://purl.org/dc/terms/>.
@prefix xsd: <http://www.w3.org/2001/XMLSchema#> .
@prefix rev:<http://purl.org/stuff/rev#> .
@prefix skos:<http://www.w3.org/2004/02/skos/core#>.


# ---------------------------------------- Metadata----------------------------------------------

<http://apps4europe.eu/vocab/odapps#>
	a owl:Ontology;
	rdfs:comment "odapps is an RDF vocabulary defined to facilitate the description of Open-Data-based ideas and applications published on the Web.";
	dct:title "The vocabulary for (L)OD ideas and applications"@en;
	dct:issued "2013-05-10"^^xsd:date;
    dct:modified "2013-07-24"^^xsd:date;
	dct:creator [foaf:mbox "Anastasia.Dimou@UGent.be"; foaf:name "Anastasia Dimou"];
	dct:creator [foaf:mbox "Pieter.Colpaert@UGent.be"; foaf:name "Pieter Colpaert"].



# ---------------------------------------- Classes ----------------------------------------------

#App Concept

odapps:AppConcept a rdfs:Class;
	rdfs:label "Application Concept" ; 
	rdfs:comment "An App Concept describes an idea for an application (a digital work) which refers to Open Data." ;
	rdfs:isDefinedBy <http://apps4europe.eu/vocab/odapps#> .


#Application
#either extending the dvia:Application or having the odapps:Application

odapps:Application a rdfs:Class;
	#dvia:Application rdfs:subClassOf odapps:Application;
	rdfs:label "Application";
	rdfs:comment "An App Concept implementation." ;
	rdfs:isDefinedBy <http://apps4eu.eu/odapps#> . 


odapps:Tool a rdfs:Class,
		owl:Class;
	rdfs:comment "The tool or library used to build the application";
	rdfs:isDefinedBy <http://apps4europe.eu/vocab/odapps#>;
	#dvia:VisualTool rdfs:subClassOf odapps:Tool ;
	rdfs:label "Tool".

# ------------------------------------ Properties ------------------------------------------------	

#odapps:consumes

odapps:consumes a rdf:Property,
		owl:ObjectProperty;
	rdfs:comment "links to the dataset used to make the application, and could be of different types or formats";
	rdfs:domain odapps:Application, odapps:AppConcept;
	rdfs:isDefinedBy <http://apps4europe.eu/vocab/odapps#>;
	rdfs:label "consumes";
	rdfs:range dcat:Dataset, xsd:string.


#datasetDescription

dvia:datasetDescription a rdf:Property;
	rdfs:comment "Property for a given descriptive informations of the datasets used for making the application. It could be used when no more details are given on the datasets like URL, formats, etc.";
	rdfs:domain odapps:AppConcept, odapps:Application;
	rdfs:isDefinedBy <http://apps4europe.eu/vocab/odapps#>;
	rdfs:label "dataset description".	


#odapps:instigator

odapps:instigator a rdf:Property;
	rdfs:label "instigator" ;
	rdfs:comment "The Agent which conceived the idea about the App Concept (the instigator/initiator)." ;
	rdfs:isDefinedBy <http://apps4europe.eu/vocab/odapps#> ;
	rdfs:domain odapps:AppConcept ;
	rdfs:range foaf:Agent .


#odapps:implements	

odapps:implements a rdf:Property ;
	rdfs:label "implements" ;
	rdfs:comment "The App Concept that this application implements" ;
	rdfs:isDefinedBy <http://apps4europe.eu/vocab/odapps#> ;
	rdfs:domain odapps:Application ;
	rdfs:range odapps:AppConcept .	


#odapps:revision

odapps:revision a rdf:Property ;	
	rdfs:label "revision of" ;
	rdfs:comment "An App concept which was revised and re-posed / extended. " ;
	rdfs:isDefinedBy <http://apps4europe.eu/vocab/odapps#> ;
	rdfs:domain odapps:AppConcept, odapps:Application ;
	rdfs:range  odapps:AppConcept, odapps:Application .
	

#odapps:theme

odapps:theme a rdf:Property ;
	rdfs:label "theme" ;
	rdfs:comment "The App Concept can be within a certain theme. " ;
	rdfs:isDefinedBy <http://apps4europe.eu/vocab/odapps#> ;
	rdfs:domain odapps:AppConcept ;
	rdfs:range skos:ConceptScheme .
	

#usesTool

odapps:usesTool a rdf:Property;
	rdfs:comment "This property links to the tools or libraries used for the application";
	rdfs:domain odapps:Application;
	rdfs:isDefinedBy <http://data.eurecom.fr/ontology/dvia>;
	rdfs:label "usesTool";
	rdfs:range odapps:Tool.


# -------------------------------------------------------------------------------------------------

#probably a broad taxonomy as the following one.
#Public administration & policy,
#Population,
#Culture/Sport/Leisure time,
#Territory,
#Health,
#Infrastructure,
#Audience (Youth/Adult/Senior),
#Environment & Nature,
#Education & Lifelong learning,
#Mobility
#Tourism,
#Safety,
#Welfare,
#Work & Economy,
#Life/Home	
	